Moved part of Quantum.thy into Misc.thy and Finite_Tensor_Product.thy

Quantum.thy
@@ -1,15 +1,15 @@
 theory Quantum
   imports Jordan_Normal_Form.Matrix_Impl "HOL-Library.Rewrite"
           Bounded_Operators.Complex_L2
+          Finite_Tensor_Products
 begin
 
 
 unbundle cblinfun_notation
 no_notation m_inv ("inv\<index> _" [81] 80)
 
-definition bra :: "'a \<Rightarrow> (_,complex) cblinfun" where "bra i = vector_to_cblinfun (ket i)*" for i
 
-instantiation mat :: (conjugate) conjugate
+(* instantiation mat :: (conjugate) conjugate
 begin
 
 definition conjugate_mat :: "'a :: conjugate mat \<Rightarrow> 'a mat"
@@ -41,19 +41,19 @@ lemma conjugate_index[simp]: \<open>i < dim_row A \<Longrightarrow> j < dim_col 
   unfolding conjugate_mat_def by auto *)
 
 lemma col_conjugate_mat[simp]: \<open>i < dim_col A \<Longrightarrow> col (conjugate A) i = conjugate (col A i)\<close>
-  unfolding conjugate_mat_def by auto
+  unfolding conjugate_mat_def by auto *)
 
-lemma sum_single: 
+(* lemma sum_single: 
   assumes "finite A"
   assumes "\<And>j. j \<noteq> i \<Longrightarrow> j\<in>A \<Longrightarrow> f j = 0"
   shows "sum f A = (if i\<in>A then f i else 0)"
   apply (subst sum.mono_neutral_cong_right[where S=\<open>A \<inter> {i}\<close> and h=f])
-  using assms by auto
+  using assms by auto *)
 
 (* lemma index_mat_fstsnd:  "fst x < nr \<Longrightarrow> snd x < nc \<Longrightarrow> mat nr nc f $$ x = f x"
   apply (cases x) by auto *)
 
-definition tensor_pack :: "nat \<Rightarrow> nat \<Rightarrow> (nat \<times> nat) \<Rightarrow> nat" where "tensor_pack X Y = (\<lambda>(x, y). x * Y + y)"
+(* definition tensor_pack :: "nat \<Rightarrow> nat \<Rightarrow> (nat \<times> nat) \<Rightarrow> nat" where "tensor_pack X Y = (\<lambda>(x, y). x * Y + y)"
 definition tensor_unpack :: "nat \<Rightarrow> nat \<Rightarrow> nat \<Rightarrow> (nat \<times> nat)"  where "tensor_unpack X Y xy = (xy div Y, xy mod Y)"
 
 lemma tensor_unpack_bound1[simp]: "i < A * B \<Longrightarrow> fst (tensor_unpack A B i) < A"
@@ -105,7 +105,7 @@ lemma tensor_unpack_sndsnd: \<open>snd (tensor_unpack B C (snd (tensor_unpack A 
 lemma tensor_unpack_fstsnd: \<open>fst (tensor_unpack B C (snd (tensor_unpack A (B * C) i)))
      = snd (tensor_unpack A B (fst (tensor_unpack (A * B) C i)))\<close>
   unfolding tensor_unpack_def apply auto
-  by (metis (no_types, lifting) Euclidean_Division.div_eq_0_iff add_0_iff bits_mod_div_trivial div_mult_self4 mod_mult2_eq mod_mult_self1_is_0 mult.commute)
+  by (metis (no_types, lifting) Euclidean_Division.div_eq_0_iff add_0_iff bits_mod_div_trivial div_mult_self4 mod_mult2_eq mod_mult_self1_is_0 mult.commute) *)
 
 type_synonym 'a state = \<open>'a ell2\<close>
 type_synonym 'a domain_end = \<open>('a state, 'a state) cblinfun\<close>
@@ -153,128 +153,6 @@ lemma maps_2hom_left: \<open>maps_2hom F2 \<Longrightarrow> maps_hom (\<lambda>a
 lemma comp_2hom: "maps_2hom timesOp"
   by (auto intro!: clinearI simp add: cbilinear_def cblinfun_apply_dist1 cblinfun_apply_dist2)
 
-lift_definition tensor_state :: \<open>'a::finite state \<Rightarrow> 'b::finite state \<Rightarrow> ('a\<times>'b) state\<close> (infixr "\<otimes>\<^sub>s" 70) is
-  \<open>\<lambda>\<psi> \<phi> (i,j). \<psi> i * \<phi> j\<close>
-  by simp
-
-lemma tensor_state_add2: \<open>tensor_state a (b + c) = tensor_state a b + tensor_state a c\<close>
-  apply transfer apply (rule ext) apply (auto simp: case_prod_beta)
-  by (meson ordered_field_class.sign_simps(42))
-
-lemma tensor_state_add1: \<open>tensor_state (a + b) c = tensor_state a c + tensor_state b c\<close>
-  apply transfer apply (rule ext) apply (auto simp: case_prod_beta)
-  by (simp add: vector_space_over_itself.scale_left_distrib)
-
-lemma tensor_state_scaleC2: \<open>tensor_state a (c *\<^sub>C b) = c *\<^sub>C tensor_state a b\<close>
-  apply transfer apply (rule ext) by (auto simp: case_prod_beta)
-
-lemma tensor_state_scaleC1: \<open>tensor_state (c *\<^sub>C a) b = c *\<^sub>C tensor_state a b\<close>
-  apply transfer apply (rule ext) by (auto simp: case_prod_beta)
-
-lemma tensor_state_inner_prod[simp]: \<open>\<langle>tensor_state a b, tensor_state c d\<rangle> = \<langle>a,c\<rangle> * \<langle>b,d\<rangle>\<close>
-  apply transfer
-  by (auto simp: case_prod_beta sum_product sum.cartesian_product mult.assoc mult.left_commute)
-
-lemma clinear_tensor_state1: "clinear (\<lambda>b. tensor_state a b)"
-  apply (rule clinearI; transfer)
-  apply (auto simp: case_prod_beta)
-  by (simp add: cond_case_prod_eta ordered_field_class.sign_simps(42))
-
-lemma clinear_tensor_state2: "clinear (\<lambda>a. tensor_state a b)"
-  apply (rule clinearI; transfer)
-  apply (auto simp: case_prod_beta)
-  by (simp add: case_prod_beta' mult.commute ordered_field_class.sign_simps(42))
-
-lemma tensor_state_ket[simp]: "tensor_state (ket i) (ket j) = ket (i,j)"
-  apply transfer by auto
-
-definition tensor_op :: \<open>('a ell2, 'b::finite ell2) cblinfun \<Rightarrow> ('c ell2, 'd::finite ell2) cblinfun
-      \<Rightarrow> (('a\<times>'c) ell2, ('b\<times>'d) ell2) cblinfun\<close> where
-  \<open>tensor_op M N = (SOME P. \<forall>a c. P *\<^sub>V (ket (a,c))
-      = tensor_state (M *\<^sub>V ket a) (N *\<^sub>V ket c))\<close>
-
-lemma tensor_op_ket: 
-  fixes a :: \<open>'a::finite\<close> and b :: \<open>'b\<close> and c :: \<open>'c::finite\<close> and d :: \<open>'d\<close>
-  shows \<open>tensor_op M N *\<^sub>V (ket (a,c)) = tensor_state (M *\<^sub>V ket a) (N *\<^sub>V ket c)\<close>
-proof -
-  define S :: \<open>('a\<times>'c) state set\<close> where "S = ket ` UNIV"
-  define \<phi> where \<open>\<phi> = (\<lambda>(a,c). tensor_state (M *\<^sub>V ket a) (N *\<^sub>V ket c))\<close>
-  define \<phi>' where \<open>\<phi>' = \<phi> \<circ> inv ket\<close>
-
-  have def: \<open>tensor_op M N = (SOME P. \<forall>a c. P *\<^sub>V (ket (a,c)) = \<phi> (a,c))\<close>
-    unfolding tensor_op_def \<phi>_def by auto
-
-  have \<open>cindependent S\<close>
-    using S_def cindependent_ket by blast
-  moreover have \<open>cspan S = UNIV\<close>
-    by (metis S_def finite_class.finite_UNIV finite_imageI ket_ell2_span span_finite_dim)
-  moreover have \<open>finite S\<close>
-    using S_def finite_class.finite_UNIV by blast
-  ultimately have "cblinfun_extension_exists S \<phi>'"
-    by (rule cblinfun_extension_exists_finite)
-  then have "\<exists>P. \<forall>x\<in>S. P *\<^sub>V x = \<phi>' x"
-    unfolding cblinfun_extension_exists_def by auto
-  then have ex: \<open>\<exists>P. \<forall>a c. P *\<^sub>V ket (a,c) = \<phi> (a,c)\<close>
-    by (metis S_def \<phi>'_def comp_eq_dest_lhs inj_ket inv_f_f rangeI)
-
-
-  then have \<open>tensor_op M N *\<^sub>V (ket (a,c)) = \<phi> (a,c)\<close>
-    unfolding def apply (rule someI2_ex[where P=\<open>\<lambda>P. \<forall>a c. P *\<^sub>V (ket (a,c)) = \<phi> (a,c)\<close>])
-    by auto
-  then show ?thesis
-    unfolding \<phi>_def by auto
-qed
-
-(* TODO should be in bounded operators (non-finite case). Implicitly proven in: *)
-thm equal_basis_0
-thm equal_ket
-thm superposition_principle_linear_ket
-lemma cbounded_linear_equal_ket:
-  fixes f g :: \<open>'a::finite ell2 \<Rightarrow> _\<close>
-  assumes \<open>clinear f\<close>
-  assumes \<open>clinear g\<close>
-  assumes \<open>\<And>i. f (ket i) = g (ket i)\<close>
-  shows \<open>f = g\<close>
-  apply (rule ext)
-  apply (rule complex_vector.linear_eq_on_span[where f=f and g=g and B=\<open>range ket\<close>])
-  using assms apply auto
-  by (metis ket_ell2_span span_finite_dim finite_class.finite_UNIV finite_imageI iso_tuple_UNIV_I) 
-
-lemma cbounded_linear_finite_ell2[simp, intro!]:
-  fixes f :: \<open>'a::finite ell2 \<Rightarrow> 'b::complex_normed_vector\<close>
-  assumes "clinear f"
-  shows \<open>cbounded_linear f\<close>
-  apply (subst cblinfun_operator_finite_dim[where basis=\<open>ket ` UNIV\<close>])
-  using assms apply (auto intro!: cindependent_ket)
-  by (metis finite_class.finite_UNIV finite_imageI iso_tuple_UNIV_I ket_ell2_span span_finite_dim)
-
-lemma tensor_op_state: "tensor_op A B *\<^sub>V tensor_state \<psi> \<phi> = tensor_state (A *\<^sub>V \<psi>) (B *\<^sub>V \<phi>)"
-proof -
-  have 1: \<open>clinear (\<lambda>a. tensor_op A B *\<^sub>V tensor_state a (ket b))\<close> for b
-    by (auto intro!: clinearI simp: tensor_state_add1 tensor_state_scaleC1 cblinfun_apply_add)
-  have 2: \<open>clinear (\<lambda>a. tensor_state (A *\<^sub>V a) (B *\<^sub>V ket b))\<close> for b
-    by (auto intro!: clinearI simp: tensor_state_add1 tensor_state_scaleC1 cblinfun_apply_add)
-  have 3: \<open>clinear (\<lambda>a. tensor_op A B *\<^sub>V tensor_state \<psi> a)\<close>
-    by (auto intro!: clinearI simp: tensor_state_add2 tensor_state_scaleC2 cblinfun_apply_add)
-  have 4: \<open>clinear (\<lambda>a. tensor_state (A *\<^sub>V \<psi>) (B *\<^sub>V a))\<close>
-    by (auto intro!: clinearI simp: tensor_state_add2 tensor_state_scaleC2 cblinfun_apply_add)
-
-  have eq_ket_ket: \<open>tensor_op A B *\<^sub>V tensor_state (ket a) (ket b) = tensor_state (A *\<^sub>V ket a) (B *\<^sub>V ket b)\<close> for a b
-    by (simp add: tensor_op_ket)
-  have eq_ket: \<open>tensor_op A B *\<^sub>V tensor_state \<psi> (ket b) = tensor_state (A *\<^sub>V \<psi>) (B *\<^sub>V ket b)\<close> for b
-    apply (rule fun_cong[where x=\<psi>])
-    using 1 2 eq_ket_ket by (rule cbounded_linear_equal_ket)
-  show ?thesis 
-    apply (rule fun_cong[where x=\<phi>])
-    using 3 4 eq_ket by (rule cbounded_linear_equal_ket)
-qed
-
-lemma comp_tensor_op: "(tensor_op a b) o\<^sub>C\<^sub>L (tensor_op c d) = tensor_op (a o\<^sub>C\<^sub>L c) (b o\<^sub>C\<^sub>L d)"
-  for a :: "'e::finite ell2 \<Rightarrow>\<^sub>C\<^sub>L 'c::finite ell2" and b :: "'f::finite ell2 \<Rightarrow>\<^sub>C\<^sub>L 'd::finite ell2" and
-  c :: "'a::finite ell2 \<Rightarrow>\<^sub>C\<^sub>L 'e ell2" and d :: "'b::finite ell2 \<Rightarrow>\<^sub>C\<^sub>L 'f ell2"
-  apply (rule equal_ket)
-  apply (rename_tac ij, case_tac ij, rename_tac i j, hypsubst_thin)
-  by (simp flip: tensor_state_ket add: tensor_op_state times_applyOp)
 
 (* lemma tensor_op_conjugate[simp]: "tensor_op (conjugate_op a) (conjugate_op b) = conjugate_op (tensor_op a b)"
   apply transfer
@@ -287,183 +165,19 @@ lemma comp_tensor_op: "(tensor_op a b) o\<^sub>C\<^sub>L (tensor_op c d) = tenso
 (* lemma tensor_op_adjoint[simp]: "tensor_op (adjoint_op a) (adjoint_op b) = adjoint_op (tensor_op a b)"
   unfolding adjoint_op_def by simp *)
 
-lemma tensor_op_adjoint: \<open>(tensor_op a b)* = tensor_op (a*) (b*)\<close>
-  apply (rule cinner_ket_adjointI[symmetric])
-  apply (auto simp flip: tensor_state_ket simp: tensor_op_state)
-  by (simp add: adjoint_I)
-
 abbreviation tensor_maps :: \<open>'a::finite domain_end \<Rightarrow> 'b::finite domain_end \<Rightarrow> ('a\<times>'b) domain_end\<close> where
   \<open>tensor_maps \<equiv> tensor_op\<close>
 
-(* TODO belongs into bounded operators *)
-lemma apply_cblinfun_distr_left: "(A + B) *\<^sub>V x = A *\<^sub>V x + B *\<^sub>V x"
-  apply transfer by simp
-
-lemma tensor_maps_cbilinear: \<open>cbilinear tensor_maps\<close>
-proof -
-  have \<open>clinear (\<lambda>b. tensor_maps a b)\<close> for a :: \<open>'a ell2 \<Rightarrow>\<^sub>C\<^sub>L 'a ell2\<close>
-    apply (rule clinearI)
-     apply (rule equal_ket, rename_tac ij, case_tac ij, rename_tac i j, hypsubst_thin)
-     apply (simp flip: tensor_state_ket add: tensor_op_state apply_cblinfun_distr_left tensor_state_add2)
-    apply (rule equal_ket, rename_tac ij, case_tac ij, rename_tac i j, hypsubst_thin)
-    by (simp flip: tensor_state_ket add: tensor_op_state apply_cblinfun_distr_left tensor_state_scaleC2)
-
-  moreover have \<open>clinear (\<lambda>a. tensor_maps a b)\<close> for b :: \<open>'b ell2 \<Rightarrow>\<^sub>C\<^sub>L 'b ell2\<close>
-    apply (rule clinearI)
-     apply (rule equal_ket, rename_tac ij, case_tac ij, rename_tac i j, hypsubst_thin)
-     apply (simp flip: tensor_state_ket add: tensor_op_state apply_cblinfun_distr_left tensor_state_add1)
-    apply (rule equal_ket, rename_tac ij, case_tac ij, rename_tac i j, hypsubst_thin)
-    by (simp flip: tensor_state_ket add: tensor_op_state apply_cblinfun_distr_left tensor_state_scaleC1)
-
-  ultimately show ?thesis
-    unfolding cbilinear_def by auto
-qed
-
 lemma tensor_2hom: \<open>maps_2hom tensor_maps\<close>
-  by (simp add: tensor_maps_cbilinear)
+  by (simp add: tensor_op_cbilinear)
 
-definition \<open>butter i j = vector_to_cblinfun (ket i) o\<^sub>C\<^sub>L (vector_to_cblinfun (ket j) :: complex \<Rightarrow>\<^sub>C\<^sub>L _)*\<close>
 
-lemma ket_Kronecker_delta: \<open>\<langle>ket i, ket j\<rangle> = (if i=j then 1 else 0)\<close>
-  by (simp add: ket_Kronecker_delta_eq ket_Kronecker_delta_neq)
-
-lemma sum_butter[simp]: \<open>(\<Sum>(i::'a::finite)\<in>UNIV. butter i i) = idOp\<close>
-  apply (rule equal_ket)
-  apply (subst complex_vector.linear_sum[where f=\<open>\<lambda>y. y *\<^sub>V ket _\<close>])
-  apply (auto simp add: apply_cblinfun_distr_left clinearI butter_def times_applyOp ket_Kronecker_delta)
-  apply (subst sum.mono_neutral_cong_right[where S=\<open>{_}\<close>])
-  by auto
-
-lemma linfun_cspan: \<open>cspan {butter i j| (i::'b::finite) (j::'a::finite). True} = UNIV\<close>
-proof (rule, simp, rule)
-  fix f :: \<open>'a ell2 \<Rightarrow>\<^sub>C\<^sub>L 'b ell2\<close>
-  have frep: \<open>f = (\<Sum>(i,j)\<in>UNIV. \<langle>ket j, f *\<^sub>V ket i\<rangle> *\<^sub>C (butter j i))\<close>
-  proof (rule cblinfun_ext)
-    fix \<phi> :: \<open>'a ell2\<close>
-    have \<open>f *\<^sub>V \<phi> = f *\<^sub>V (\<Sum>i\<in>UNIV. butter i i) *\<^sub>V \<phi>\<close>
-      by auto
-    also have \<open>\<dots> = (\<Sum>i\<in>UNIV. f *\<^sub>V butter i i *\<^sub>V \<phi>)\<close>
-      apply (subst (2) complex_vector.linear_sum)
-       apply (simp add: cblinfun_apply_add clinearI plus_cblinfun.rep_eq)
-      by simp
-    also have \<open>\<dots> = (\<Sum>i\<in>UNIV. (\<Sum>j\<in>UNIV. butter j j) *\<^sub>V f *\<^sub>V butter i i *\<^sub>V \<phi>)\<close>
-      by simp
-    also have \<open>\<dots> = (\<Sum>i\<in>UNIV. \<Sum>j\<in>UNIV. butter j j *\<^sub>V f *\<^sub>V butter i i *\<^sub>V \<phi>)\<close>
-      apply (subst (3) complex_vector.linear_sum)
-       apply (simp add: cblinfun_apply_add clinearI plus_cblinfun.rep_eq)
-      by simp
-    also have \<open>\<dots> = (\<Sum>(i,j)\<in>UNIV. butter j j *\<^sub>V f *\<^sub>V butter i i *\<^sub>V \<phi>)\<close>
-      by (simp add: sum.cartesian_product)
-    also have \<open>\<dots> = (\<Sum>(i,j)\<in>UNIV. \<langle>ket j, f *\<^sub>V ket i\<rangle> *\<^sub>C (butter j i *\<^sub>V \<phi>))\<close>
-      by (simp add: butter_def times_applyOp mult.commute)
-    also have \<open>\<dots> = (\<Sum>(i,j)\<in>UNIV. \<langle>ket j, f *\<^sub>V ket i\<rangle> *\<^sub>C (butter j i)) *\<^sub>V \<phi>\<close>
-      unfolding applyOp_scaleC1[symmetric] case_prod_beta
-      thm complex_vector.linear_sum
-      apply (subst complex_vector.linear_sum[where f=\<open>\<lambda>x. x *\<^sub>V \<phi>\<close>])
-       apply (simp add: apply_cblinfun_distr_left clinearI)
-      by simp
-    finally show \<open>f *\<^sub>V \<phi> = (\<Sum>(i,j)\<in>UNIV. \<langle>ket j, f *\<^sub>V ket i\<rangle> *\<^sub>C (butter j i)) *\<^sub>V \<phi>\<close>
-      by -
-  qed
-  show \<open>f \<in> cspan {butter i j |i j. True}\<close>
-    apply (subst frep)
-    apply (auto simp: case_prod_beta)
-    by (metis (mono_tags, lifting) complex_vector.span_base complex_vector.span_scale complex_vector.span_sum mem_Collect_eq)
-qed
-
-ML \<open>
+(* ML \<open>
 \<^term>\<open>{f x y | x y. P x y}\<close>
-\<close>
+\<close> *)
 
+(* TODO: move tensor stuff into Finite_Tensor_Product *)
 
-lemma linfun_cindependent: \<open>cindependent {butter i j| (i::'b::finite) (j::'a::finite). True}\<close>
-proof (rule independent_if_scalars_zero)
-  show finite: \<open>finite {butter (i::'b) (j::'a) |i j. True}\<close>
-    apply (subst (6) conj.left_neutral[symmetric])
-    apply (rule finite_image_set2)
-    by auto
-  fix f :: \<open>('a ell2 \<Rightarrow>\<^sub>C\<^sub>L 'b ell2) \<Rightarrow> complex\<close> and g :: \<open>'a ell2 \<Rightarrow>\<^sub>C\<^sub>L 'b ell2\<close>
-  define lin where \<open>lin = (\<Sum>g\<in>{butter i j |i j. True}. f g *\<^sub>C g)\<close>
-  assume \<open>lin = 0\<close>
-  assume \<open>g \<in> {butter i j |i j. True}\<close>
-  then obtain i j where g: \<open>g = butter i j\<close>
-    by auto
-  (* define bra :: "'b \<Rightarrow> (_,complex) cblinfun" where "bra i = vector_to_cblinfun (ket i)*" for i *)
-
-  have *: "bra i *\<^sub>V f g *\<^sub>C g *\<^sub>V ket j = 0"
-    if \<open>g\<in>{butter i j |i j. True} - {butter i j}\<close> for g 
-  proof -
-    from that
-    obtain i' j' where g: \<open>g = butter i' j'\<close>
-      by auto
-    from that have \<open>g \<noteq> butter i j\<close> by auto
-    with g consider (i) \<open>i\<noteq>i'\<close> | (j) \<open>j\<noteq>j'\<close>
-      by auto
-    then show \<open>bra i *\<^sub>V f g *\<^sub>C g *\<^sub>V ket j = 0\<close>
-    proof cases
-      case i
-      then show ?thesis 
-        unfolding g by (auto simp: butter_def times_applyOp bra_def ket_Kronecker_delta_neq)
-    next
-      case j
-      then show ?thesis
-        unfolding g by (auto simp: butter_def times_applyOp ket_Kronecker_delta_neq)
-    qed
-  qed
-
-  have \<open>0 = bra i *\<^sub>V lin *\<^sub>V ket j\<close>
-    using \<open>lin = 0\<close> by auto
-  also have \<open>\<dots> = (\<Sum>g\<in>{butter i j |i j. True}. bra i *\<^sub>V (f g *\<^sub>C g) *\<^sub>V ket j)\<close>
-    unfolding lin_def
-    apply (rule complex_vector.linear_sum)
-    by (simp add: cblinfun_apply_add clinearI plus_cblinfun.rep_eq)
-  also have \<open>\<dots> = (\<Sum>g\<in>{butter i j}. bra i *\<^sub>V (f g *\<^sub>C g) *\<^sub>V ket j)\<close>
-    apply (rule sum.mono_neutral_right)
-    using finite * by auto
-  also have \<open>\<dots> = bra i *\<^sub>V (f g *\<^sub>C g) *\<^sub>V ket j\<close>
-    by (simp add: g)
-  also have \<open>\<dots> = f g\<close>
-    unfolding g 
-    by (auto simp: butter_def times_applyOp bra_def ket_Kronecker_delta_eq)
-  finally show \<open>f g = 0\<close>
-    by simp
-qed
-
-lemma tensor_butter: \<open>tensor_op (butter i j) (butter k l) = butter (i,k) (j,l)\<close>
-  for i :: "_" and j :: "_::finite" and k :: "_" and l :: "_::finite"
-  apply (rule equal_ket, case_tac x)
-  apply (auto simp flip: tensor_state_ket simp: times_applyOp tensor_op_state butter_def)
-  by (auto simp: tensor_state_scaleC1 tensor_state_scaleC2)
-
-lemma cspan_tensor_op: \<open>cspan {tensor_op (butter i j) (butter k l)| i (j::_::finite) k (l::_::finite). True} = UNIV\<close>
-  unfolding tensor_butter
-  apply (subst linfun_cspan[symmetric])
-  by (metis surj_pair)
-
-lemma cindependent_tensor_op: \<open>cindependent {tensor_op (butter i j) (butter k l)| i (j::_::finite) k (l::_::finite). True}\<close>
-  unfolding tensor_butter
-  using linfun_cindependent
-  by (smt (z3) Collect_mono_iff complex_vector.independent_mono)
-
-
-lemma tensor_extensionality:
-  fixes F G :: \<open>('a::finite\<times>'b::finite, 'c) maps_hom\<close>
-  assumes [simp]: "maps_hom F" "maps_hom G"
-  assumes tensor_eq: "(\<And>a b. F (tensor_op a b) = G (tensor_op a b))"
-  shows "F = G"
-proof (rule ext, rule complex_vector.linear_eq_on_span[where f=F and g=G])
-  show \<open>clinear F\<close> and \<open>clinear G\<close>
-    using assms by (simp_all add: cbilinear_def)
-  show \<open>x \<in> cspan  {tensor_op (butter i j) (butter k l)| i j k l. True}\<close> 
-    for x :: \<open>('a \<times> 'b) ell2 \<Rightarrow>\<^sub>C\<^sub>L ('a \<times> 'b) ell2\<close>
-    using cspan_tensor_op by auto
-  show \<open>F x = G x\<close> if \<open>x \<in> {tensor_maps (butter i j) (butter k l) |i j k l. True}\<close> for x
-    using that by (auto simp: tensor_eq)
-qed
-
-lemma tensor_id[simp]: \<open>tensor_maps idOp idOp = idOp\<close>
-  apply (rule equal_ket, case_tac x)
-  by (simp flip: tensor_state_ket add: tensor_op_state)
 
 definition tensor_lift :: \<open>('a::finite, 'b::finite, 'c) maps_2hom \<Rightarrow> (('a\<times>'b, 'c) maps_hom)\<close> where
   "tensor_lift F2 = (SOME G. clinear G \<and> (\<forall>a b. G (tensor_maps a b) = F2 a b))"
@@ -482,11 +196,11 @@ proof -
     obtain i' j' k' l' where y: "y = (i',j',k',l')" by (meson prod_cases4) 
     have 1: "bra (i,k) *\<^sub>V t4 x *\<^sub>V ket (j,l) = 1"
       by (auto simp: bra_def t4_def x tensor_op_state butter_def times_applyOp ket_Kronecker_delta_eq
-               simp flip: tensor_state_ket)
+               simp flip: tensor_ell2_ket)
     assume \<open>x \<noteq> y\<close>
     then have 2: "bra (i,k) *\<^sub>V t4 y *\<^sub>V ket (j,l) = 0"
       by (auto simp: bra_def t4_def x y tensor_op_state butter_def times_applyOp ket_Kronecker_delta_neq
-               simp flip: tensor_state_ket)
+               simp flip: tensor_ell2_ket)
     from 1 2 that
     show False
       by auto
@@ -519,7 +233,7 @@ proof -
     apply (rule complex_vector.linear_eq_on_span[where g=\<open>\<lambda>a. F2 a _\<close> and B=\<open>{butter k l|k l. True}\<close>])
     unfolding linfun_cspan
     using * apply (auto intro!: linear_compose[unfolded o_def, where f=\<open>\<lambda>a. tensor_maps a _\<close> and g=\<open>(*\<^sub>V) G\<close>])
-    apply (metis cbilinear_def tensor_maps_cbilinear)
+    apply (metis cbilinear_def tensor_op_cbilinear)
     apply (simp add: cblinfun_apply_add clinearI)
     using assms unfolding cbilinear_def by blast
   have G_F2: \<open>G *\<^sub>V tensor_maps a b = F2 a b\<close> for a b
@@ -527,7 +241,7 @@ proof -
     unfolding linfun_cspan
     using * apply (auto simp: cblinfun_apply_add clinearI
                         intro!: linear_compose[unfolded o_def, where f=\<open>tensor_maps a\<close> and g=\<open>(*\<^sub>V) G\<close>])
-    apply (meson cbilinear_def tensor_maps_cbilinear)
+    apply (meson cbilinear_def tensor_op_cbilinear)
     using assms unfolding cbilinear_def by blast
 
   have \<open>clinear F2' \<and> (\<forall>a b. F2' (tensor_maps a b) = F2 a b)\<close>
@@ -562,30 +276,30 @@ lift_definition assoc_state' :: \<open>('a::finite\<times>('b::finite\<times>'c:
   apply (rule clinearI; transfer)
   by auto
 
-lemma assoc_state_tensor: \<open>assoc_state *\<^sub>V tensor_state (tensor_state a b) c = tensor_state a (tensor_state b c)\<close>
+lemma assoc_state_tensor: \<open>assoc_state *\<^sub>V tensor_ell2 (tensor_ell2 a b) c = tensor_ell2 a (tensor_ell2 b c)\<close>
   apply (rule cbounded_linear_equal_ket[THEN fun_cong, where x=a])
-    apply (simp add: cblinfun_apply_add clinearI tensor_state_add1 tensor_state_scaleC1)
-   apply (simp add: clinear_tensor_state2)
+    apply (simp add: cblinfun_apply_add clinearI tensor_ell2_add1 tensor_ell2_scaleC1)
+   apply (simp add: clinear_tensor_ell22)
   apply (rule cbounded_linear_equal_ket[THEN fun_cong, where x=b])
-    apply (simp add: cblinfun_apply_add clinearI tensor_state_add1 tensor_state_add2 tensor_state_scaleC1 tensor_state_scaleC2)
-   apply (simp add: clinearI tensor_state_add1 tensor_state_add2 tensor_state_scaleC1 tensor_state_scaleC2)
+    apply (simp add: cblinfun_apply_add clinearI tensor_ell2_add1 tensor_ell2_add2 tensor_ell2_scaleC1 tensor_ell2_scaleC2)
+   apply (simp add: clinearI tensor_ell2_add1 tensor_ell2_add2 tensor_ell2_scaleC1 tensor_ell2_scaleC2)
   apply (rule cbounded_linear_equal_ket[THEN fun_cong, where x=c])
-    apply (simp add: cblinfun_apply_add clinearI tensor_state_add2 tensor_state_scaleC2)
-   apply (simp add: clinearI tensor_state_add2 tensor_state_scaleC2)
+    apply (simp add: cblinfun_apply_add clinearI tensor_ell2_add2 tensor_ell2_scaleC2)
+   apply (simp add: clinearI tensor_ell2_add2 tensor_ell2_scaleC2)
   unfolding assoc_state.rep_eq
   apply transfer
   by auto
 
-lemma assoc_state'_tensor: \<open>assoc_state' *\<^sub>V tensor_state a (tensor_state b c) = tensor_state (tensor_state a b) c\<close>
+lemma assoc_state'_tensor: \<open>assoc_state' *\<^sub>V tensor_ell2 a (tensor_ell2 b c) = tensor_ell2 (tensor_ell2 a b) c\<close>
   apply (rule cbounded_linear_equal_ket[THEN fun_cong, where x=a])
-    apply (simp add: cblinfun_apply_add clinearI tensor_state_add1 tensor_state_scaleC1)
-   apply (simp add: clinearI tensor_state_add1 tensor_state_scaleC1)
+    apply (simp add: cblinfun_apply_add clinearI tensor_ell2_add1 tensor_ell2_scaleC1)
+   apply (simp add: clinearI tensor_ell2_add1 tensor_ell2_scaleC1)
   apply (rule cbounded_linear_equal_ket[THEN fun_cong, where x=b])
-    apply (simp add: cblinfun_apply_add clinearI tensor_state_add1 tensor_state_add2 tensor_state_scaleC1 tensor_state_scaleC2)
-   apply (simp add: clinearI tensor_state_add1 tensor_state_add2 tensor_state_scaleC1 tensor_state_scaleC2)
+    apply (simp add: cblinfun_apply_add clinearI tensor_ell2_add1 tensor_ell2_add2 tensor_ell2_scaleC1 tensor_ell2_scaleC2)
+   apply (simp add: clinearI tensor_ell2_add1 tensor_ell2_add2 tensor_ell2_scaleC1 tensor_ell2_scaleC2)
   apply (rule cbounded_linear_equal_ket[THEN fun_cong, where x=c])
-    apply (simp add: cblinfun_apply_add clinearI tensor_state_add2 tensor_state_scaleC2)
-   apply (simp add: clinearI tensor_state_add2 tensor_state_scaleC2)
+    apply (simp add: cblinfun_apply_add clinearI tensor_ell2_add2 tensor_ell2_scaleC2)
+   apply (simp add: clinearI tensor_ell2_add2 tensor_ell2_scaleC2)
   unfolding assoc_state'.rep_eq
   apply transfer
   by auto
@@ -600,7 +314,7 @@ lemma assoc_hom: \<open>maps_hom assoc\<close>
 lemma assoc_apply: \<open>assoc (tensor_maps (tensor_maps a b) c) = tensor_maps a (tensor_maps b c)\<close>
   apply (rule equal_ket)
   apply (case_tac x)
-  by (simp add: assoc_def times_applyOp tensor_op_state assoc_state_tensor assoc_state'_tensor flip: tensor_state_ket)
+  by (simp add: assoc_def times_applyOp tensor_op_state assoc_state_tensor assoc_state'_tensor flip: tensor_ell2_ket)
 
 
 definition lvalue :: \<open>('a, 'b) maps_hom \<Rightarrow> bool\<close> where
